src/Ext/Expr.v
@@ -4,7 +4,7 @@ Require Import MirrorCore.Ext.ExprD.
 Require Export MirrorCore.Ext.ExprT.
 Require Export MirrorCore.Ext.ExprFacts.
 Require Export MirrorCore.Ext.ExprLift.
+Require Export MirrorCore.Ext.ExprTactics.
 (*
 Require Export MirrorCore.Ext.ExprSubst.
-Require Export Mirrorcore.Ext.ExprSimplify.
 *)
